esercitazione.lean
@@ -1,6 +1,0 @@
-import Lean
-open Lean Meta Server Widget
-
-def name := "Hi"
-
-#eval s!"\{'kind':'hyp','name':'','type':'}'}"
