newFile.lean
@@ -1,2 +1,0 @@
-theorem foo : True := by
-  let x := 3
